Primitive_Matchers/Common_Primitive_Syntax.thy
@@ -11,12 +11,12 @@ text{*Primitive Match Conditions which only support interfaces, IPv4 addresses, 
 datatype_new common_primitive =
   is_Src: Src (src_sel: ipt_ipv4range) | 
   is_Dst: Dst (dst_sel: ipt_ipv4range) |
-  IIface iface |
-  OIface iface |
-  Prot protocol | 
+  is_Iiface: IIface (iiface_sel: iface) |
+  is_Oiface: OIface (oiface_sel: iface) |
+  is_Prot: Prot (prot_sel: protocol) | 
   is_Src_Ports: Src_Ports (src_ports_sel: ipt_ports) | 
   is_Dst_Ports: Dst_Ports (dst_ports_sel: ipt_ports) | 
-  Extra string
+  is_Extra: Extra (extra_sel: string)
 
 
 
@@ -24,7 +24,10 @@ lemma wf_disc_sel_common_primitive[simp]:
       "wf_disc_sel (is_Src_Ports, src_ports_sel) Src_Ports"
       "wf_disc_sel (is_Dst_Ports, dst_ports_sel) Dst_Ports"
       "wf_disc_sel (is_Src, src_sel) Src"
-      "wf_disc_sel (is_Dst, dst_sel) Dst"
+      "wf_disc_sel (is_Iiface, iiface_sel) IIface"
+      "wf_disc_sel (is_Oiface, oiface_sel) OIface"
+      "wf_disc_sel (is_Prot, prot_sel) Prot"
+      "wf_disc_sel (is_Extra, extra_sel) Extra"
   by(simp_all add: wf_disc_sel.simps)
 
 
